Progress

theories/Dot/misc_unused/dot_lty.v
@@ -1,17 +1,12 @@
 From iris.proofmode Require Import tactics.
 From D Require Export iris_prelude.
-From D Require Import ty_interp_subst_lemmas lty.
+From D Require Import lty ty_interp_subst_lemmas pty_interp_subst_lemmas.
 From D.Dot Require Import syn syn.path_repl dlang_inst path_wp lr_syn_aux.
 From D.pure_program_logic Require Import lifting.
 
 Notation "'λI' x .. y , t" := (fun x => .. (fun y => t%I) ..)
   (at level 200, x binder, y binder, right associativity, only parsing,
   format "'[  ' '[  ' 'λI'  x  ..  y ']' ,  '/' t ']'") : function_scope.
-
-Include TyInterpLemmas VlSorts dlang_inst.
-
-(** Override notation from [dlang] to specify scope. *)
-Notation "⟦ T ⟧" := (ty_interp T%ty).
 
 Implicit Types (Σ : gFunctors).
 Implicit Types
@@ -21,6 +16,13 @@ Implicit Types
 Module SemTypes.
 
 Include LtyJudgements VlSorts dlang_inst.
+Include PTyInterpLemmas VlSorts dlang_inst.
+Import persistent_ty_interp_lemmas.
+
+(** Override notations to specify scope. *)
+Notation "p⟦ T ⟧" := (pty_interp T%ty).
+
+Notation "p⟦ Γ ⟧*" := (pty_interp <$> Γ).
 
 Record dlty Σ := Dlty {
   dlty_label : label;
@@ -32,9 +34,11 @@ Global Arguments dlty_car {_} !_ _ /.
 
 Local Notation IntoPersistent' P := (IntoPersistent false P P).
 
-Section Defs.
-  Context `{HdotG: dlangG Σ} {i : nat}.
-  Implicit Types (φ : hoEnvD Σ i) (τ : olty Σ i).
+Definition dslty Σ := env -> iPPred dms Σ.
+Notation Dslty T := (λ ρ, IPPred (λI ds, T ρ ds)).
+
+Section defs.
+  Context `{HdotG: dlangG Σ}.
   Implicit Types (T : olty Σ 0) (TD : dlty Σ).
   Definition mkDlty l (φ : envPred dm Σ) `{∀ ρ d, Persistent (φ ρ d)} : dlty Σ :=
     Dlty l (λ ρ, IPPred (φ ρ)).
@@ -42,18 +46,25 @@ Section Defs.
   Definition lift_dlty (φ : dlty Σ) l : envPred dm Σ :=
     λI ρ d, ⌜ dlty_label φ = l ⌝ ∧ φ ρ d.
 
-  (* Definition sdtp Γ l (φ : dlty Σ) d : iProp Σ :=
-    □∀ ρ, ⌜path_includes (pv (ids 0)) ρ [(l, d)] ⌝ → s⟦Γ⟧* ρ → lift_dlty φ l ρ d.|[ρ]. *)
-
-  Definition sdtp Γ TD l d : iProp Σ :=
+  (* Definition sdtp Γ TD l d : iProp Σ :=
     (⌜ l = dlty_label TD ⌝ ∧
-      □∀ ρ, s⟦Γ⟧* ρ → TD ρ d.|[ρ])%I.
+      □∀ ρ, s⟦Γ⟧* ρ → TD ρ d.|[ρ])%I. *)
+  Definition sdtp Γ (φ : dlty Σ) l d : iProp Σ :=
+    □∀ ρ, ⌜path_includes (pv (ids 0)) ρ [(l, d)] ⌝ → s⟦Γ⟧* ρ → lift_dlty φ l ρ d.|[ρ].
   Global Arguments sdtp /.
+
+  (** Multi-definition typing *)
+  Definition sdstp Γ (T : dslty Σ) ds : iProp Σ :=
+    ⌜wf_ds ds⌝ ∧ □∀ ρ, ⌜path_includes (pv (ids 0)) ρ ds ⌝ → s⟦Γ⟧* ρ → T ρ ds.|[ρ].
+  Global Arguments sdstp /.
 
   Definition sptp Γ T p i: iProp Σ :=
     □∀ ρ, s⟦Γ⟧* ρ -∗
       ▷^i path_wp (p.|[ρ]) (λ v, oClose T ρ v).
+  Global Arguments sptp /.
 
+  Context {i : nat}.
+  Implicit Types (φ : hoEnvD Σ i) (τ : olty Σ i).
   (*
     Even if semantic types use infinite substitutions, we can still reuse the
     current stamping theory, based on finite substitutions.
@@ -65,7 +76,7 @@ Section Defs.
 
   Definition dm_to_type d i (ψ : hoD Σ i) : iProp Σ :=
     (∃ s σ, ⌜ d = dtysem σ s ⌝ ∧ s ↗n[ σ , i ] ψ)%I.
-End Defs.
+End defs.
 
 Notation "Γ s⊨ {  l := d  } : T" := (sdtp Γ T l d) (at level 64, d, l, T at next level).
 Notation "Γ s⊨p p : τ , i" := (sptp Γ τ p i) (at level 74, p, τ, i at next level).
@@ -153,14 +164,9 @@ Section SemTypes.
 
   Definition oPrim b : olty Σ 0 := olty0 (λI ρ v, ⌜pure_interp_prim b v⌝).
 
-  Class PersTyInterp (ty : Type) Σ :=
-    pers_ty_interp : ty → olty Σ 0.
-  Notation "p⟦ T ⟧" := (pers_ty_interp T%ty).
-  Global Arguments pers_ty_interp {_ _ _} !_ /.
-
-  Global Instance pinterp : PersTyInterp ty Σ :=
+  Global Instance pinterp : PTyInterp ty Σ :=
     fix pinterp (T : ty) : olty Σ 0 :=
-    let _ := pinterp : PersTyInterp ty Σ in
+    let _ := pinterp : PTyInterp ty Σ in
     match T with
     | TTMem l L U => oTTMem l p⟦ L ⟧ p⟦ U ⟧
     | TVMem l T' => oTVMem l p⟦ T' ⟧
@@ -175,67 +181,49 @@ Section SemTypes.
     | TSel p l => oTSel p l
     | TSing p => oPSing p
     end.
-  (* Wrap this into ty_interp to reuse lemmas. *)
-  Global Instance pers_to_ty_interp : TyInterp ty Σ := flip pers_ty_interp vnil.
-  Global Arguments pers_to_ty_interp _ /.
-  Global Arguments ty_interp {_ _ _} _ /.
-
-  Global Instance interp_lemmas: TyInterpLemmas ty Σ.
+  Global Instance pinterp_lemmas: PTyInterpLemmas ty Σ.
   Proof.
-    split => /=; induction T => sb1 sb2 w /=;
+    split => /=; induction T => args sb1 sb2 w /=;
       properness; rewrite ?scons_up_swap ?hsubst_comp; trivial; by f_equiv => ?.
   Qed.
 
-  Global Instance interp_persistent T ρ v : Persistent (⟦ T ⟧ ρ v) := _.
+  (* Strong sealing. *)
+  Definition BAD_LABEL : label. Proof. exact "". Qed.
 
   Fixpoint def_interp_base (T : ty) : dlty Σ :=
     match T with
     | TTMem l L U => oDTMem l p⟦ L ⟧ p⟦ U ⟧
     | TVMem l T' => oDVMem l p⟦ T' ⟧
-    | _ => mkDlty "" (λI _ _, False)
+    | _ => mkDlty BAD_LABEL (λI _ _, False)
     end.
-
-  Global Instance def_interp_persistent T ρ d :
-    Persistent (def_interp_base T ρ d).
-  Proof. destruct T; try apply _. Qed.
 
   Definition def_interp T l := lift_dlty (def_interp_base T) l.
 
-  Definition defs_interp_and (interp1 interp2 : envPred dms Σ) : envPred dms Σ :=
-    λI ρ ds, interp1 ρ ds ∧ interp2 ρ ds.
+  (* Definition Dslty' {Σ} (T : envPred dms Σ)
+   `{∀ ρ ds, Persistent (T ρ ds)} : env -> iPPred dms Σ := Dslty T. *)
 
-  Definition lift_dinterp_dms T : envPred dms Σ := λI ρ ds,
-    ∃ l d, ⌜ dms_lookup l ds = Some d ⌝ ∧ def_interp T l ρ d.
+  Program Definition defs_interp_and (interp1 interp2 : dslty Σ) : dslty Σ :=
+    Dslty (λI ρ ds, interp1 ρ ds ∧ interp2 ρ ds).
 
-  Fixpoint defs_interp T : envPred dms Σ :=
+  Definition lift_dinterp_dms (T : dlty Σ) : dslty Σ := Dslty (λI ρ ds,
+    ∃ l d, ⌜ dms_lookup l ds = Some d ⌝ ∧ lift_dlty T l ρ d).
+
+  Fixpoint defs_interp T : dslty Σ :=
     match T with
     | TAnd T1 T2 => defs_interp_and (defs_interp T1) (defs_interp T2)
-    | TTop => λI ρ ds, True
-    | _ => lift_dinterp_dms T
+    | TTop => Dslty (λI ρ ds, True)
+    | _ => lift_dinterp_dms (def_interp_base T)
     end.
 
-  Global Instance defs_interp_persistent T ρ ds : Persistent (defs_interp T ρ ds).
-  Proof. induction T; try apply _. Qed.
-
-  (** Multi-definition typing *)
-  Definition idstp Γ T ds : iProp Σ :=
-    ⌜wf_ds ds⌝ ∧ □∀ ρ, ⌜path_includes (pv (ids 0)) ρ ds ⌝ → s⟦Γ⟧* ρ → defs_interp T ρ ds.|[ρ].
-  Global Arguments idstp /.
-
-  (* Fixpoint interp_env (Γ : ctx) (ρ : var → vl) : iProp Σ :=
-    match Γ with
-    | T :: Γ' => interp_env Γ' (stail ρ) ∧ ⟦ T ⟧ ρ (shead ρ)
-    | nil => True
-    end%I. *)
-
-  Notation "p⟦ Γ ⟧*" := (pers_ty_interp <$> Γ).
   Notation "d⟦ T ⟧" := (def_interp_base T%ty).
+  Notation "ds⟦ T ⟧" := (defs_interp T%ty).
 
   Definition idtp  Γ T l d     := sdtp  p⟦Γ⟧* d⟦T⟧ l d.
-  (* Definition idstp Γ T ds      := sdstp p⟦Γ⟧* p⟦T⟧ ds. *)
+  Definition idstp Γ T ds : iProp Σ := sdstp p⟦Γ⟧* ds⟦ T ⟧ ds.
   Definition ietp  Γ T e       := setp  p⟦Γ⟧* p⟦T⟧ e.
   Definition istpi Γ T1 T2 i j := sstpi p⟦Γ⟧* p⟦T1⟧ p⟦T2⟧ i j.
   Definition iptp  Γ T p i     := sptp  p⟦Γ⟧* p⟦T⟧ p i.
+  (* Global Arguments idstp /. *)
 
   Global Instance idtp_persistent Γ T l d: IntoPersistent' (idtp Γ T l d) | 0 := _.
   Global Instance idstp_persistent Γ T ds: IntoPersistent' (idstp Γ T ds) | 0 := _.
@@ -243,43 +231,59 @@ Section SemTypes.
   Global Instance istpi_persistent Γ T1 T2 i j : IntoPersistent' (istpi Γ T1 T2 i j) | 0 := _.
   Global Instance iptp_persistent Γ T p i : IntoPersistent' (iptp Γ T p i) | 0 := _.
 
-  Implicit Types (T : olty Σ 0) (TD : dlty Σ).
+  Implicit Types (T : olty Σ 0) (Td : dlty Σ) (Tds : dslty Σ).
 
-  Local Notation IntoPersistent' P := (IntoPersistent false P P).
   (* Avoid auto-dropping box (and unfolding) when introducing judgments persistently. *)
-  Global Instance sdtp_persistent Γ TD l d: IntoPersistent' (sdtp Γ TD l d) | 0 := _.
-  (* Global Instance sdstp_persistent Γ T ds: IntoPersistent' (sdstp Γ T ds) | 0 := _. *)
+  Local Notation IntoPersistent' P := (IntoPersistent false P P).
+  Global Instance sdtp_persistent Γ Td l d: IntoPersistent' (sdtp Γ Td l d) | 0 := _.
+  Global Instance sdstp_persistent Γ Tds ds: IntoPersistent' (sdstp Γ Tds ds) | 0 := _.
   Global Instance setp_persistent Γ T e : IntoPersistent' (setp Γ T e) | 0 := _.
   Global Instance sstpi_persistent Γ T1 T2 i j : IntoPersistent' (sstpi Γ T1 T2 i j) | 0 := _.
   Global Instance sptp_persistent Γ T p i : IntoPersistent' (sptp Γ T p i) | 0 := _.
-
 End SemTypes.
+Notation "d⟦ T ⟧" := (def_interp_base T%ty).
+Notation "ds⟦ T ⟧" := (defs_interp T%ty).
+
 Notation "d ↗ ψ" := (dm_to_type 0 d ψ) (at level 20).
-Notation "p⟦ T ⟧" := (pers_ty_interp T%ty).
-Notation "p⟦ Γ ⟧*" := (pers_ty_interp <$> Γ).
-Notation "p⟦ T ⟧ₑ" := (interp_expr ⟦ T ⟧).
-(* Notation "⟦ T ⟧ₑ" := (interp_expr p⟦ T ⟧). *)
-(* Definition interp_env (Γ : ctx) : env -d> iPropO Σ := env_oltyped (pers_ty_interp <$> Γ).
-Global Arguments interp_env !_ _ /.
-Notation "⟦ Γ ⟧*" := (interp_env Γ). *)
-(* Notation "⟦ Γ ⟧*" := (env_oltyped (pers_ty_interp <$> Γ)). *)
+Notation "p⟦ T ⟧ₑ" := (interp_expr p⟦ T ⟧).
 Notation "⟦ Γ ⟧*" := s⟦ p⟦ Γ ⟧* ⟧*.
 
+(* Notation "⟦ T ⟧ₑ" := (interp_expr p⟦ T ⟧). *)
+(* Definition interp_env (Γ : ctx) : env -d> iPropO Σ := env_oltyped (pty_interp <$> Γ).
+Global Arguments interp_env !_ _ /.
+Notation "⟦ Γ ⟧*" := (interp_env Γ). *)
+(* Notation "⟦ Γ ⟧*" := (env_oltyped (pty_interp <$> Γ)). *)
 
 (** Single-definition typing *)
-Notation "Γ ⊨ {  l := d  } : T" := (idtp p⟦Γ⟧* p⟦T⟧ l d) (at level 74, d, l, T at next level).
+Notation "Γ ⊨ {  l := d  } : T" := (idtp Γ T l d) (at level 74, d, l, T at next level).
 (** Multi-definition typing *)
-Notation "Γ ⊨ds ds : T" := (idstp p⟦Γ⟧* p⟦T⟧ ds) (at level 74, ds, T at next level).
+Notation "Γ ⊨ds ds : T" := (idstp Γ T ds) (at level 74, ds, T at next level).
 (** Expression typing *)
-Notation "Γ ⊨ e : T" := (ietp p⟦Γ⟧* p⟦T⟧ e) (at level 74, e, T at next level).
-Notation "Γ ⊨p p : T , i" := (iptp p⟦Γ⟧* p⟦T⟧ p i) (at level 74, p, T, i at next level).
+Notation "Γ ⊨ e : T" := (ietp Γ T e) (at level 74, e, T at next level).
+Notation "Γ ⊨p p : T , i" := (iptp Γ T p i) (at level 74, p, T, i at next level).
+Notation "Γ ⊨ T1 , i <: T2 , j " := (istpi Γ T1 T2 i j) (at level 74, T1, T2, i, j at next level).
 
-Notation "Γ ⊨ T1 , i <: T2 , j " := (istpi p⟦Γ⟧* p⟦T1⟧ p⟦T2⟧ i j) (at level 74, T1, T2, i, j at next level).
+Import stamp_transfer.
+(** Single-definition typing *)
+Notation "Γ ⊨[ gφ  ] { l := d  } : T" := (wellMappedφ gφ → idtp Γ T l d)%I (at level 74, d, l, T at next level).
+(** Multi-definition typing *)
+Notation "Γ ⊨ds[ gφ  ] ds : T" := (wellMappedφ gφ → idstp Γ T ds)%I (at level 74, ds, T at next level).
+(** Expression typing *)
+Notation "Γ ⊨[ gφ  ] e : T" := (wellMappedφ gφ → ietp Γ T e)%I (at level 74, e, T at next level).
+Notation "Γ ⊨p[ gφ  ] p : T , i" := (wellMappedφ gφ → iptp Γ T p i)%I (at level 74, p, T, i at next level).
+Notation "Γ ⊨[ gφ  ] T1 , i <: T2 , j" := (wellMappedφ gφ → istpi Γ T1 T2 i j)%I (at level 74, T1, T2, i, j at next level).
 
 Section SampleTypingLemmas.
   Context `{HdotG: dlangG Σ}.
-
   Implicit Types (τ L T U : olty Σ 0).
+
+  Lemma def_interp_tvmem_eq l T p ρ :
+    lift_dlty (oDVMem l T) l ρ (dpt p) ⊣⊢
+    path_wp p (oClose T ρ).
+  Proof.
+    rewrite /lift_dlty/=; iSplit. by iDestruct 1 as (_ pmem [= ->]) "$".
+    iIntros "H"; iSplit; first done; iExists p. by auto.
+  Qed.
 
   Lemma Sub_Sel Γ L U va l i:
     Γ s⊨ tv va : oTTMem l L U, i -∗
@@ -305,17 +309,16 @@ Section SampleTypingLemmas.
     iApply "HψU" => //. iNext. by iRewrite "Hag".
   Qed.
 
-  Lemma D_Typ_Abs Γ T L U s σ l :
-    Γ s⊨ T, 1 <: U, 1 -∗
-    Γ s⊨ L, 1 <: T, 1 -∗
+  Lemma D_Typ_Abs Γ T L U s σ l:
+    Γ s⊨ oLater T, 0 <: oLater U, 0 -∗
+    Γ s⊨ oLater L, 0 <: oLater T, 0 -∗
     s ↝[ σ ] T -∗
     Γ s⊨ { l := dtysem σ s } : oDTMem l L U.
   Proof.
-    iIntros "#HTU #HLT #Hs /="; iSplit => //.
-    iIntros "!>" (ρ) "#Hg /=".
+    iIntros "#HTU #HLT #Hs /= !>" (ρ Hpid) "#Hg"; iSplit => //=.
     iDestruct "Hs" as (φ Hγφ) "Hγ".
     iExists (hoEnvD_inst (σ.|[ρ]) φ); iSplit.
-    by iApply dm_to_type_intro.
+    by iApply (dm_to_type_intro with "Hγ").
     iModIntro; repeat iSplit; iIntros (v) "#HL"; rewrite later_intuitionistically.
     - iIntros "!>". iApply Hγφ. by iApply "HLT".
     - iApply "HTU" => //. by iApply Hγφ.
@@ -327,4 +330,26 @@ Section SampleTypingLemmas.
   Proof. iIntros "#Hs"; iApply D_Typ_Abs; by [| iIntros "!> **"]. Qed.
 End SampleTypingLemmas.
 
+Module ty_compat.
+  Include TyInterpLemmas VlSorts dlang_inst.
+  Notation "⟦ T ⟧" := (ty_interp T%ty).
+
+  Section defs.
+    Context `{HdotG: dlangG Σ}.
+    (* Wrap this into ty_interp to reuse lemmas. *)
+    Global Instance pto_ty_interp : TyInterp ty Σ := flip pty_interp vnil.
+    Global Instance interp_persistent T ρ v : Persistent (⟦ T ⟧ ρ v) := _.
+
+    Global Arguments pto_ty_interp _ /.
+    Global Arguments ty_interp {_ _ _} _ /.
+
+    Global Instance interp_lemmas: TyInterpLemmas ty Σ.
+    Proof. split => /= *; apply persistent_ty_interp_lemmas.interp_subst_compose_ind. Qed.
+
+    Lemma def_interp_tvmem_eq' l (T : ty) p ρ:
+      def_interp (TVMem l T) l ρ (dpt p) ⊣⊢
+      path_wp p (⟦ T ⟧ ρ).
+    Proof. apply def_interp_tvmem_eq. Qed.
+  End defs.
+End ty_compat.
 End SemTypes.
