theories/pty_interp_subst_lemmas.v
@@ -1,0 +1,61 @@
+From D Require Import prelude asubst_base dlang.
+From iris.proofmode Require Import tactics.
+
+From D Require Import lty.
+Module Type PTyInterpLemmas (Import VS : VlSortsFullSig) (Import LWP : LiftWp VS)
+  (Import LJ : LtyJudgements VS LWP).
+
+Module persistent_ty_interp_lemmas.
+
+Class PTyInterp ty Σ :=
+  pty_interp : ty -> olty Σ 0.
+Notation "p⟦ T ⟧" := (pty_interp T).
+Notation "p⟦ g ⟧g" := (fmap (M := gmap stamp) pty_interp g).
+
+(* Also appears in Autosubst. *)
+Global Arguments pty_interp {_ _ _} !_ /.
+
+Class PTyInterpLemmas ty Σ `{sort_ty : Sort ty} `{!PTyInterp ty Σ} := {
+  interp_subst_compose_ind T {args} ρ1 ρ2 v:
+    p⟦ T.|[ρ1] ⟧ args ρ2 v ⊣⊢ p⟦ T ⟧ args (ρ1 >> ρ2) v;
+}.
+
+(** * Lemmas about the logical relation itself. *)
+Section logrel_binding_lemmas.
+  Context `{Htil : PTyInterpLemmas ty Σ}.
+
+  Implicit Types
+          (L T U: ty) (v: vl) (e: tm) (ρ : env).
+
+  Lemma interp_subst_compose T {args} ρ1 ρ2 ρ3:
+    ρ1 >> ρ2 = ρ3 → p⟦ T.|[ρ1] ⟧ args ρ2 ≡ p⟦ T ⟧ args ρ3.
+  Proof. move=> <- v. exact: interp_subst_compose_ind. Qed.
+
+  Lemma interp_weaken_one τ ρ {args} :
+     p⟦ shift τ ⟧ args ρ ≡ p⟦ τ ⟧ args (stail ρ).
+  Proof. apply interp_subst_compose. autosubst. Qed.
+
+  Lemma interp_subst_one T v w ρ {args} :
+    p⟦ T.|[v/] ⟧ args ρ w ≡ p⟦ T ⟧ args (v.[ρ] .: ρ) w.
+  Proof. apply interp_subst_compose. autosubst. Qed.
+
+  Lemma interp_subst_ids T ρ {args} : p⟦ T ⟧ args ρ ≡ p⟦ T.|[ρ] ⟧ args ids.
+  Proof. symmetry. apply interp_subst_compose. autosubst. Qed.
+
+  (**
+    We have, unconditionally, that
+    p⟦ T.|[∞ σ] ⟧ args ρ = p⟦ T ⟧ args (∞ σ >> ρ).
+
+    But [∞ σ >> ρ] and [∞ σ.|[ρ]] are only equal for
+    [length σ] entries.
+  *)
+  Lemma interp_subst_commute T σ ρ v (HclT : nclosed T (length σ)) args :
+    p⟦ T.|[∞ σ] ⟧ args ρ v ≡ p⟦ T ⟧ args (∞ σ.|[ρ]) v.
+  Proof.
+    rewrite interp_subst_compose_ind !(interp_subst_ids T _ _) -hsubst_comp.
+    (* *The* step requiring [HclT]. *)
+    by rewrite (subst_compose _ _ HclT).
+  Qed.
+End logrel_binding_lemmas.
+End persistent_ty_interp_lemmas.
+End PTyInterpLemmas.
